rocq/rec/extensions.v
@@ -1,0 +1,159 @@
+Require Export rec.typing.
+
+Import typing.Notations.
+Import reduction.Notations.
+
+(** Syntax extensions *)
+
+(** We can define abbreviations for "normal" lambda calculus terms, 
+    which do not include value restrictions, by using eagerlet *)
+
+Import FinValues.
+
+(** eager let *) 
+
+Definition eagerlet {n} (e1 : Tm n) (e2 : Tm (S n)) :=
+  match e1 with 
+  | ret v => e2[v..]
+  | _ => let_ e1 e2
+  end.
+
+Lemma t_eagerlet {n} Γ :
+  forall (e1 : Tm n) (e2 : Tm (S n)) (τ1 τ2 : Ty 0), 
+    Γ |-e e1 ∈ τ1 -> τ1 .: Γ |-e e2 ∈ τ2 -> Γ |-e eagerlet e1 e2 ∈ τ2.
+Proof. 
+  intros. unfold eagerlet.
+  unfold eagerlet. intros. destruct e1; eauto. inversion H.
+  eapply substitution_tm; eauto with rec.
+  all: eauto with rec.
+Qed.
+
+Lemma eagerlet_subst {m n : nat} (sigma : fin n -> Val m) (e1 : Tm n) (e2 : Tm (S n)) :
+   (eagerlet e1 e2)[sigma] = eagerlet (e1[sigma]) (e2[up_Val_Val sigma]).
+Proof. 
+  destruct e1; cbn; try reflexivity. now asimpl.
+Qed.
+
+Lemma ms_eagerlet_cong (e1 e1' : Tm 0) (e2 : Tm 1) :
+  e1 ~>* e1' -> eagerlet e1 e2 ~>* eagerlet e1' e2.
+Proof.
+  intro h. unfold eagerlet.
+  destruct e1. apply ret_steps_to_itself in h. rewrite h. eapply ms_refl.
+  all: destruct e1'.
+  all: try solve [eapply ms_let_cong; eauto].
+  all: eapply ms_app; [ eapply ms_let_cong; eauto| eapply ms_one; econstructor ].
+Qed.  
+
+
+(* ------------------ Application -----------------  *)
+
+Definition app_tm {n} (e1 e2 : Tm n) : Tm n := 
+  eagerlet e1 (eagerlet e2⟨↑⟩ (app (var f1) (var f0))).
+
+
+Lemma t_app_tm {n} Γ (e1 e2: Tm n) τ1 τ2 : 
+    Γ |-e e1 ∈ (Arr τ1 τ2) -> Γ |-e  e2 ∈ τ1 ->
+    Γ |-e (app_tm e1 e2) ∈ τ2.
+Proof. 
+  intros. unfold app_tm.
+  eapply t_eagerlet; eauto with renaming rec.
+  eapply t_eagerlet; eauto with renaming rec.
+  repeat (econstructor; eauto with renaming rec).
+Qed.
+
+
+Lemma s_app_tm_cong1 (e1 e1' e2 : Tm 0) :
+  e1 ~>* e1' -> app_tm e1 e2 ~>* app_tm e1' e2.
+Proof. intro h.  unfold app_tm. eapply ms_eagerlet_cong; auto. 
+Qed.
+
+
+Lemma s_app_tm_cong2 v1 (e2 e2' : Tm 0) :
+  e2 ~>* e2' -> app_tm (ret v1) e2 ~>* app_tm (ret v1) e2'.
+Proof. 
+  intro h.
+  unfold app_tm. 
+  asimpl.
+  unfold eagerlet at 1 3.
+  repeat rewrite eagerlet_subst.
+  eapply ms_eagerlet_cong.
+  asimpl.
+  auto.
+Qed.
+
+
+(* ----------------- Products ---------------------- *)
+
+Definition prod_tm {n} (e1 e2 : Tm n) : Tm n := 
+  eagerlet e1 (eagerlet e2⟨↑⟩ (ret (prod (var f1) (var f0)))).
+Definition prj_tm {n} b (e1 : Tm n) : Tm n := 
+  eagerlet e1 (prj b (var f0)).
+
+(** Typing rules for extended product syntax *)
+
+Definition t_prod_tm {n} (Γ : Ctx n) e1 e2 τ1 τ2 : 
+    Γ |-e e1 ∈ τ1 ->   Γ |-e e2 ∈ τ2 -> 
+    Γ |-e prod_tm e1 e2 ∈ Prod τ1 τ2.
+Proof.
+  intros. unfold prod_tm.
+  eapply t_eagerlet; eauto with renaming rec.
+  eapply t_eagerlet; eauto with renaming rec.
+Qed.
+
+Definition s_prod_cong1 e1 e1' e2 :
+  e1 ~>* e1' ->
+  prod_tm e1 e2 ~>* prod_tm e1' e2.
+Proof.
+  intro h.
+  unfold prod_tm.
+  eapply ms_eagerlet_cong; eauto.
+Qed.
+
+Definition s_prod_cong2 v1 e2 e2' :
+  e2 ~>* e2' ->
+  prod_tm (ret v1) e2 ~>* prod_tm (ret v1) e2'.
+Proof.
+  intro h.
+  unfold prod_tm.
+  unfold eagerlet at 1 3.
+  repeat rewrite eagerlet_subst.
+  eapply ms_eagerlet_cong.
+  asimpl.
+  done.
+Qed.
+
+Lemma t_prj1_tm {n} Γ (e:Tm n) τ1 τ2 : 
+  Γ |-e e ∈  Prod τ1 τ2 -> 
+  Γ |-e prj_tm true e ∈ τ1.
+Proof.
+  intros h. unfold prj_tm.
+  eapply t_eagerlet; eauto with renaming rec.
+  econstructor; eauto with rec.
+  eapply t_var'. cbn. eauto.  
+Qed.
+
+
+Lemma t_prj2_tm {n} Γ (e:Tm n) τ1 τ2 : 
+  Γ |-e e ∈  Prod τ1 τ2 -> 
+  Γ |-e prj_tm false e ∈ τ2.
+Proof.
+  intros h. unfold prj_tm.
+  eapply t_eagerlet; eauto with renaming rec.
+  econstructor; eauto with rec.
+  eapply t_var'. cbn. eauto.  
+Qed.
+
+
+Definition s_prj_cong b e1 e1' :
+  e1 ~>* e1' ->
+  prj_tm b e1 ~>* prj_tm b e1'.
+Proof.
+  intro h.
+  unfold prj_tm.
+  eapply ms_eagerlet_cong; eauto.
+Qed.
+
+
+
+
+
